src/Std/Data/DHashMap/Internal/WF.lean
@@ -407,14 +407,8 @@ theorem getₘ_eq_getValue [BEq α] [Hashable α] [LawfulBEq α] {m : Raw₀ α 
 
 theorem getEntryₘ_eq_getEntry [BEq α] [EquivBEq α] [Hashable α] [LawfulHashable α] {m : Raw₀ α β} (hm : Raw.WFImp m.1)
     {a : α} {h : m.containsₘ a} :
-    m.getEntryₘ a h = List.getEntry a (toListModel m.1.buckets) (containsₘ_eq_containsKey hm ▸ h) := by
-  apply apply_bucket_with_proof hm a AssocList.getEntry List.getEntry
-  · intro a' l h
-    apply AssocList.getEntry_eq
-  · intro l l' a' h hd hp
-    apply getEntry_of_perm hd hp
-  · intro l l' a' h₁ h₂
-    apply getEntry_append_of_containsKey_eq_false h₂
+    m.getEntryₘ a h = List.getEntry a (toListModel m.1.buckets) (containsₘ_eq_containsKey hm ▸ h) :=
+  apply_bucket_with_proof hm a AssocList.getEntry List.getEntry AssocList.getEntry_eq getEntry_of_perm getEntry_append_of_containsKey_eq_false
 
 theorem get_eq_getValueCast [BEq α] [Hashable α] [LawfulBEq α] {m : Raw₀ α β} (hm : Raw.WFImp m.1)
     {a : α} {h : m.contains a} :
